\topic{Cauchy's LDE}

General form:

$$
	a_{0} x^{n} \cdot \frac{d^{n} y}{d x^{n}}+a_{1} x^{n-1} \frac{d^{n-1} y}{d x^{n-1}}+\cdots+a_{x} x^{d y} d x+y=\phi(x)
$$

is reduced to LDE with Const. coett by substituting

\begin{flalign*}
	 & x=e^{t} \text{, or } t=\ln (x) \quad \frac{d}{d t}=D, \because x^2 \cdot \frac{d^{2} y}{d x^2 } \Rightarrow D(D-1) y \\
	 & x \frac{d y}{d x}=D y \quad: \quad x^{3} \frac{d^{3} y}{d x^{3}} \rightarrow D(D-1)(D-2) y
\end{flalign*}

Solve:

1). $x^2 \cdot \frac{d^{2} y}{d x^2 }-x \frac{d y}{d x}+y=\ln (x)$

This if Cauchy's LDG $\therefore$ put $x=e^{t}, \Rightarrow \sin(x)=t$

Redue to LDE with const-eoeth.

\begin{flalign*}
	\text{ (1) } \rightarrow & D(D-1) y-D y+y=t                                \\
	                         & \left(D^{2}-2 D+1\right) y=t                    \\
	                         & \therefore C F=\left(c_{1}+c_{2} t\right) e^{t}
\end{flalign*}

\begin{flalign*}
	 & P_{I}=\frac{t}{(D-1)^{2}} \rightarrow                               \\
	 & = \frac{t}{D^{2}-2 D+1}=\left(1+\left(D^{2}-2 D\right)\right)^{-2}= \\
	 & =\left(1-D^{2}+2 D\right) t                                         \\
	 & =t+2                                                                \\
	 & =\ln (x)+2
\end{flalign*}

$\therefore$ solution: $y=\left(c_{1}+c_{2} \ln (x)\right) e^{\ln (x)}+\ln (x)+2$

\begin{flalign*}
	 & \left.=\oint_{1}+r_{2} \ln (x)\right] x+\ln (x)+2 \\
	 & =c_{1} x+\ln (x)\left(1+x c_{2}\right)+2
\end{flalign*}

\begin{enumerate}
	\setcounter{enumi}{1}
	\item $x^2 \cdot y^{\prime \prime}-4 x y'+6 y=x^2 $
\end{enumerate}

put $x=e^{t}, t=\ln (x)$

\begin{flalign*}
	 & D(D-1) y-4 D y+6 y=e^{2 t}                                              \\
	 & \left(D^{2}-5 D+6\right) y=e^{2 t}                                      \\
	 & D=\frac{e^{2 t}}{D^{2}-5 D+6}, \quad C F=c_{1} e^{+3 x}+c_{2} e^{-12 x} \\
	 & \therefore P I_{1}=2                                                    \\
	 & \Rightarrow \frac{e^{2 t}}{4-10+6}=
\end{flalign*}

\begin{flalign*}
	 & \frac{+5 \pm \sqrt{25-25}}{2}=\frac{+5 \pm 1}{2}                                            \\
	 & =+2,-3                                                                                      \\
	 & \frac{e^{2 t}}{(D-3)(D-2)} \Rightarrow \frac{1}{D-2} \cdot \frac{t e^{2 t}}{D-3}=-t e^{2 t}
\end{flalign*}

$\therefore$ Solution: $y=c_{1} e^{3 t}+c_{2} e^{2 t}+t e^{2 t}$

$$
	=c_{1} e^{\ln (x)^{2}}+c_{2} e^{2 \cdot \ln (x)}-\ln (x) e^{2 \ln (x)}
$$

\begin{flalign*}
	  & =c_{1} x^{3}+c_{2} x^2 -\ln (x) x^2         \\
	y & =c_{1} x^{3}+x^2 \left(c_{2}-\ln (x)\right)
\end{flalign*}

HT\\
3. $x^2 y^{\prime \prime}-2 x y'-4 y=x^{4}$.\\
4. $x^2 y^{\prime \prime}+4 x y'+2 y=x^2 +x^{-2}$

In 10\\
H.
