\topic{Exact Differential Equation}
\begin{itemize}
	\item A Differential equation of the form $M(x, y) d x+N(x, y) d y=0$ is sard to be exact differential equation.
\end{itemize}

such that $\frac{\partial \mu}{\partial x}=m(x, y), \& \frac{\partial \mu}{\partial y}=N(x, y)$

ie, $M d x+N d y=\frac{\partial \mu}{\partial x} d x+\frac{\partial \mu}{\partial y} d y=d \mu$

$$
	\therefore \text{ Solution is } \int d \mu \Rightarrow \mu(x, y)=c
$$

Methnd to find exact or not

\begin{itemize}
	\item If Diff. eqn. is exact then $\frac{\partial M}{\partial y}=\frac{\partial N}{\partial x}$
\end{itemize}

eg: $(1-x) \cdot d x-(1+y) d y=0$

$M=1-x, \quad N=-(1+y)$

$\frac{\partial M}{\partial y}=0, \quad \frac{\partial N}{\partial x}=0 \quad \Rightarrow \frac{\partial M}{\partial y}=\frac{\partial N}{\partial x} \quad \therefore$ Eqn. is exact.

Method to solve E.D.E

Solution: $\int M d x+\int[$ Terms in $N$ not containing $x] d y=c$

Solve $(1-x) d g-(1+y) d y=0$

A) Solution: $\int(1-x) d x+\int-(1+y) d y=c / 2 \quad$ (soy $)$

$$
	\begin{gathered}
		x-\frac{x^2 }{2}-y-\frac{y^2}{2}=c / 2 \\
		\Rightarrow \quad x-y=\frac{x^2 +y^2}{2}+c / 2 \\
		2(x-y)=x^2 +y^2+c
	\end{gathered}
$$

\begin{enumerate}
	\setcounter{enumi}{1}
	\item $\left(3 x^2 +4 x y\right) d x+\left(2 x^2 +2 y\right) d y=0$
\end{enumerate}

\begin{flalign*}
	 & M=3 x^2 +4 x y, \quad \frac{\partial M}{\partial y}=4 x                                                                                                          \\
	 & N=2 x^2 +2 y \quad, \quad \frac{\partial N}{\partial x}=4 x \quad \frac{\partial M}{\partial y}=\frac{\partial N}{\partial x} \Rightarrow \text{ eqn. is Exact }
\end{flalign*}

Solution: $\int M \cdot d x+\int[$ terms in $N$ not containing $x] d y=c$

$$
	\begin{gathered}
		\int\left(3 x^2 +4 x y\right) d x+\int 2 y \cdot d y=c \\
		x^{3}+2 x^2 y+y^2=c
	\end{gathered}
$$

\begin{enumerate}
	\setcounter{enumi}{2}
	\item Why condition for exactness is $\frac{\partial M}{\partial x}=\frac{\partial N}{\partial y}$ ?
\end{enumerate}

A) for \href{http://E.DE}{E.DE}. $\exists u(x, y): \frac{\partial u}{\partial y}=N(x, y) \cdot \frac{\partial u}{\partial x}=m(x, y)$

consider $\frac{\partial^{2} u}{\partial x \partial y}=\frac{\partial N}{\partial x}, \quad \frac{\partial^{2} u}{\partial y \partial x}=\frac{\partial M}{\partial y}$

since. $u(x, y)$ represents a family of curve and

it is continuous, $\frac{\partial^{2} u}{\partial x \partial y}=\frac{\partial^{2} u}{\partial y \partial x} \Rightarrow \frac{\partial M}{\partial y}=\frac{\partial N}{\partial x}$

\begin{enumerate}
	\setcounter{enumi}{1}
	\item Anodian woy]:
\end{enumerate}

$m=3 x^2 +4 x y,(1) \quad N=2 x^2 +2 y-(2)$

$\frac{\partial M}{\partial H}$ $=4 x$

$\nrightarrow \cdot m$ $0,4 x y+\Psi(x)$

$=4 x y+\psi(x)-15$

comparing (1) \& (3) $\psi(x)=3 x^2 $

\begin{enumerate}
	\setcounter{enumi}{3}
	\item $\left(2 x \cos(y)+3 x^2 y\right) d x+\left(x^{3}-x^2 \sin y-y\right) d y=0$
\end{enumerate}

$$
	\begin{array}{ll}
		M=2 x \cos(y)+3 x^2 y                              & N=x^{3}-x^2 \sin(y)-y                            \\
		\frac{\partial M}{\partial y}=-2 x \sin(y)+3 x^2 , & \frac{\partial N}{\partial x}=3 x^2 -2 x \sin(y) \\
		\frac{\partial M}{\partial y}=\frac{\partial N}{\partial x} \Rightarrow \text{ eqn. is EDE }
	\end{array}
$$

Solution: $\int\left(2 x \cos(y)+3 x^2 y\right) d x+\int-y d y \pm c$

$$
	x^2 \cos(y)+x^{3} y-\frac{y^2}{2}=c
$$

Hw:

\begin{enumerate}
	\item Solve:
\end{enumerate}

\begin{flalign*}
	 & \text{ a) }\left(5 x^{4}+3 x^2 y^2-2 x y^{3}\right) d x+\left(2 x^{3} y-3 x^2 y^2-5 y^{4}\right) d y=0 \\
	 & \text{ b) }(2 x y+y-\tan(y)) d x+\left(x^2 -x \tan ^{2}(y)+\sec ^{2}(y)+2 y\right) d y=0
\end{flalign*}

\begin{enumerate}
	\setcounter{enumi}{1}
	\item (another uy).
\end{enumerate}

$$
	M=3 x^2 +4 x y, N=2 x^2 +2 y
$$

Define $f(x, y)$ f $f_{x}=m . f_{y}=N$

Then solution is given by $f(x, y)=c_{1}$

\begin{enumerate}
	\item Integrate $f_{x}$ \href{http://with respect toge}{with respect toge} to find $f(x, y)$ :
\end{enumerate}

$$
	f(x, y)=\int\left(3 x^2 +4 y x\right) d x=x^{3}+2 x^2 y+\psi(y) \quad
$$

Differentiate this curty to find $\psi(y)$ :

$$
	\partial f_{y}=2 x^2 +\frac{d \psi}{d y}
$$

Substitute $f_{y}=N, \quad$ (by $\left.d e f.\right)$

$$
	2 x^2 +\frac{d \psi}{d y}=2 x^2 +2 y \Rightarrow \frac{d \psi}{d y}=2 y
$$

Integrate $d \psi$ sixy urty: $\psi(y)=y^2$

substitute $\psi(y)$ in $f(x, y)$ :

$$
	f(x, y)=x^{3}+y^2+2 x^2 y
$$

The Solution is $f(x, y)=c$ :

$$
	\begin{gathered}
		: \frac{x^{3}+y^2+2 x^2 y=c}{2} \\
		x^{4}+y^2+2 x^2 y=x^{4}-x^{3}+c \\
		\Rightarrow\left(y+x^2 \right)^{2}=x^{4}-x^{3}+c \\
		y+x^2 = \pm \sqrt{x^{4}+x^{3}+c} \\
		y=-x^2 \pm \sqrt{x^{4}-x^{3}+c}
	\end{gathered}
$$


$? \frac{d y^{4}}{d x}+\frac{x y}{1-x^2 }=x \sqrt{y}$

divide by $\sqrt{y}$.


\begin{equation*}
	y^{-1 / 2} \frac{d y}{d x}+\frac{x y^{1 / 2}}{1-x^2 }=x \tag{1}
\end{equation*}


let $z=y^{1 / 2}, \quad \frac{d z}{d x}=\frac{1}{2} y^{-1 / 2} \frac{d y}{d x}$

$\therefore$ (1) become:

$$
	\frac{d z}{d x}+\underbrace{\frac{d x}{2\left(1-x^2 \right)}}_{p} \cdot z=\frac{1}{2} x \text{. }
$$

let $f=e^{\frac{1}{e} \int \frac{x}{1-x^2 } d x}=\left(1-x^2 \right)^{-1 / 4} \quad-\frac{1}{2} \int \frac{x}{1-x^2 } d x$ $t=1-x^2 $ $d t=d x \cdot(-2 x)$


\begin{align*}
	s: \mathbb{Z} \cdot F=\int Q \cdot F \cdot d x+c & =-2 x \cdot d x                                                                                                               \\
	\Psi \cdot\left(1-x^2 \right)^{-1 / 4}           & =\int \frac{1}{2} x \cdot\left(1-x^2 \right)^{-1 / 4} d x+c \quad-\frac{1}{4} \int \frac{d t}{t} \Rightarrow \Rightarrow n(t) \\
	                                                 & =\quad \frac{1}{2} \int x \cdot\left(1-x^2 \right)^{-1 / 4} d x+c \quad \text{ - (2) }
\end{align*}


$\therefore$ Solution is: $y \cdot F=\int Q \cdot F \cdot d x+c$

let $t=1-x^2 , d t=-2 x d x$

$\therefore$ (2) becomes:

\begin{flalign*}
	y \cdot\left(1-x^2 \right)^{-1 / 4} & =-\frac{1}{4} \int t^{-1 / 4} d t+c                                       \\
	                                    & =-\frac{1}{4} x \frac{t^{3 / 4}}{-1 / 4+1}=-\frac{1}{3} \cdot t^{3 / 4}+c \\
	z \cdot\left(1-x^2 \right)^{-1 / 4} & =-\frac{1}{3}\left(1-x^2 \right)^{3 / 4}+c                                \\
	z                                   & =-\frac{1}{3}\left(1-x^2 \right)+c \cdot\left(1-x^2 \right)^{1 / 4}
\end{flalign*}

$$
	\begin{gathered}
		z=\sqrt{y} \\
		\therefore y=\left[\sqrt[4]{c \cdot\left(1-x^2 \right)}-\frac{1}{3}\left(1-x^2 \right)\right]^{2} \\
		\frac{d y}{d x}+x \cdot \sin(2 y)=x^{3} \cdot \cos ^{2}(y) \\
		\equiv \frac{d y}{d x}+x \cdot 2 \cdot \sin(y) \cos(y)=x^{3} \cdot \cos ^{2}(y)
	\end{gathered}
$$

Divide by $\cos ^{2}(y)$ :

$$
	\sec ^{2}(y) \cdot \frac{d y}{d x}+2 x \cdot \tan(y)=x^{3}
$$

let $z=\tan(y)=\frac{d z}{d x}=\sec ^{2}(y) \cdot \frac{d y}{d x}$.

$$
	\frac{d z}{d x}+2 x \cdot z=x^{3}
$$

I.F $=e^{\sqrt{2 x}}=e^{x^2 }$, \&multiply by it:

\begin{flalign*}
	e^{x^2 } \frac{d z}{d x}           & +2 x \cdot e^{x^2 } \cdot z=x^{3} \cdot e^{x^2 }  \\
	\Rightarrow \quad e^{x^2 } \cdot z & =\int x^{3} \cdot e^{x^2 } d x^{+}+c              \\
	                                   & =\frac{1}{2} e^{x^2 }\left(x^2 -1\right)+c        \\
	\therefore \tan(y)                 & =\frac{1}{2}\left(x^2 -1\right)+e^{-x^2 } \cdot c
\end{flalign*}

\begin{enumerate}
	\setcounter{enumi}{2}
	\item $\frac{d y}{d x}+y \tan(x)=y^{3} \cdot \sec (x)$
\end{enumerate}

EDE -Hw-1

\begin{flalign*}
	 & \underbrace{\left(5 x^{4}+3 x^2 y^2-2 x y^{3}\right)}_{M} d x+\underbrace{\left(2 x^{3} y-3 x^2 y^2-5 y^{4}\right)}_{N} d y=0 \\
	 & M_{x y}=6 x^2 y-6 x y^2, N_{y}=6 x^2 y-6 x y^2                                                                                \\
	 & M_{y}=N_{y} \quad \therefore \text{ EDE }
\end{flalign*}

$\therefore$ So ln: $\int_{\text{cor }} m d x+\int(N \not x) d x y=C$

$$
	=x^{5}-y^{5}+x^{3} y^2-x^2 y^{3}=c
$$

$29 / 9$

$$
	\left(3 x^2 +6 x y^2\right) d x+\left(6 x^2 y+4 y^{3}\right) d y=0
$$

Solve:\\
a) $[\cos(x) \tan(y)+\cos(x+y)] d x+\left[\sin(x) \cdot \sec ^{2}(y)+\cos(x+y)\right] d y=0$\\
A) $M=\cos(x) \tan(y)+\cos(x+y) \cdot \frac{\partial M}{\partial y}=\cos(x) \cdot \sec ^{2}(y)-\sin(x+y)$

$$
	N=\sin(x) \sec ^{2}(y)+\cos(x+y), \frac{\partial N}{\partial x}=\sec ^{2}(y) \cdot \cos(x)-\sin(x+y)
$$

$\frac{\partial M}{\partial y}=\frac{\partial r}{\partial x} \Rightarrow$ Equation is exact.

$\therefore$ Solution is:

\begin{flalign*}
	 & \int_{y \cdot \text{ cons }} M \cdot d x+\underbrace{\int(\operatorname{tem} s \operatorname{in} N \text{ not containing } x) d y}_{0} d=c \\
	 & \tan(y) \int \cos(x) d x+\int \cos(x+y) d x \quad=c                                                                                        \\
	 & \tan(y) \cdot \sin(x)+\sin(x+y)=c
\end{flalign*}

\begin{enumerate}
	\item $(y \cos(x)+1) d x+\sin(x) d y=0$

	\item $\left(\sec (x) \tan(x) \tan(y)-e^{x}\right) d x+\left(\sec (x) \sec ^{2}(y) d y=0\right.$

\end{enumerate}
