\section*{Partial Differentiation}
If $z=f(x, y)$ it can be differentiated partially wort $x$ ory $\frac{\partial z}{\partial x}=\lim _{\Delta x \rightarrow 0} \frac{f(x+\Delta x, y)-f(x, y)}{\Delta x}$, Here we treat $y$ as constant $z_{x}=\frac{\partial z}{\partial x}$

e.y: $z(x, y)=x^2 +y^2+2 x y$,

$z_{y}=\frac{\partial z}{\partial x}$ $\frac{\partial z}{\partial x}=2 x+0+2 y \quad 0$

or wirt. $y$ by: $\frac{\partial z}{\partial y}=\lim _{\Delta y \rightarrow 0} \frac{f(x, y+\Delta y)-f(x, y)}{\Delta y}$ [we treat $x$ constaint] $\frac{\partial z}{\partial y}=0+2 y+2 x$

find $\frac{\partial f}{\partial x} \& \frac{\partial f}{\partial y}$ in following:\\
a) $f(x, y)=x^{3}+3 x^2 y+x y^{3}$\\
A) $\frac{\partial f}{\partial x}=3 x^2 +6 x y+y^{3} \quad, \frac{\partial f}{\partial y}=0+3 x^2 +3 x y^2$\\
b) $f(x, y)=2 x \cos(y)+3 x^2 y$\\
A) $\frac{\partial f}{\partial x}=2 \cos(y)+6 x y \quad \frac{\partial f}{\partial y}=-2 x \sin(y)+3 x^2 $

C) \begin{flalign*}
	f(x, y) & =x \tan ^{-1}\left(\frac{y}{x}\right)                                                                                                                                       \\
	f_{x}   & =\frac{1}{1+y^2 / x^2 } \cdot \frac{\partial}{\partial x} \cdot\left(\frac{y}{x}\right)=\frac{y}{x^2 } \cdot \frac{x^2 }{x^2 +y^2} \cdot-\frac{1}{x^2 }=\frac{-y}{x^2 +y^2}
\end{flalign*}

$\Delta f_{y}=\frac{1}{1+y^2 / x^2 } \cdot \frac{\partial}{\partial y}\left(\frac{y}{x}\right)=\frac{x^2 }{x^2 +y^2} \cdot \frac{1}{x}=\frac{x}{x^2 +y^2}$\\
d) $f(x, y)=x^{3}-x^2 \sin(y)-y$

$f_{x}=3 x^2 -2 x \sin(y) . \quad f_{y}=-x^2 \cos(y)-1$


\section*{Higher Order Partial Derivative}
\begin{itemize}
	\item $\frac{\partial^{2} f}{\partial x^2 }=\frac{\partial}{\partial x}\left(\frac{\partial f}{\partial x}\right)=f_{x x}$
	\item $\frac{\partial^{2} f}{\partial y^2}=\frac{\partial}{\partial y}\left(\frac{\partial f}{\partial y}\right)=f_{y y}$
\end{itemize}

$\cdot \frac{\partial^{2} f}{\partial x \partial y}=\frac{\partial}{\partial x}\left(\frac{\partial f}{\partial y}\right)=f_{x y}$

\begin{itemize}
	\item $\frac{\partial^{2} f}{\partial y \partial x}=\frac{\partial}{\partial y}\left(\frac{\partial f}{\partial x}\right)=f_{y x}$
\end{itemize}

\begin{itemize}
	\item If $f(x, y)$ is continuous function, $f_{x y}=f_{y x}$
\end{itemize}

\begin{enumerate}
	\item find I \& II order partial derivatives of\\
	      a) $t=x^2 y$\\
	      A) $f_{x}=2 x y$. $f_{y}=x^2 , f_{x y}=2 x, f_{y x}=2 x, f_{x x}=2 y, f_{y y}=0$\\
	      b) $x^{3} f(x, y)=x^{3} \sin(y)$
\end{enumerate}

$f_{x}=3 x^2 \sin(y), f_{x x}=6 x \sin(y), f_{y x}=3 x^2 \cos(y)$

$f_{y}=x^{3} \cos(y), \quad f_{y y}=-x^{3} \sin(y), \quad f_{x y}=-3 x^2 \sin(y)$

\section*{Differentials}
If $z=f(x, y), d z, d x, d y$ are known as differentials. in $z, z, y$ respectively.

cex $d z=\frac{\partial z}{\partial x} d x+\frac{\partial z}{\partial y} d y$

1.) find the differentiols in $f$ of if $f=\frac{x^{3}}{3}-x y^2$

$$
	\begin{array}{r}
		d f=\frac{d f}{\partial x} \frac{\partial f}{\partial x} d x+\frac{\partial f}{\partial y} d y \\
		d f=\left(x^2 -y^2\right) d x-2 x y d y
	\end{array}
$$
