\topic{Simultaneous LDE}

It contains two or more dependent variables (soy $x, y .$. and one inclependent variable (say $t$ )

\begin{enumerate}
	\item $\quad \frac{d x}{d t}=7 x-y, \quad \frac{d x}{d t}-\frac{d y}{d t}=5(x-y)$\\
	      A)
\end{enumerate}


\begin{align*}
	 & \frac{d x}{d t}-2 x=y=0 \rightarrow(D-7) x+y=0  \tag{1}                                   \\
	 & \frac{d x}{d t}-\frac{d y}{5 x}-\frac{d y}{d x}+5 y=0 \leadsto(D-5) x+-(D-5) y=0  \tag{2} \\
	 & (D-5) \times 0:                                                                           \\
	 & (D-7)(D-5) x+(D-5) y=0                                                                    \\
	 & +[(D-5) \dot{x}-(D-5) y=0]                                                                \\
	 & \underbrace{\left(D^{2}-11 D+30\right)}_{\text{aux ff }} x=0                              \\
	 & =                                                                                         \\
	 & \therefore \text{ costs of aux ff } z                                                     \\
	 & 5,6                                                                                       \\
	 & \therefore C \cdot F_{12} x=C, e^{5 t}+C_{2} e^{6 t}
\end{align*}


$$
	D=\frac{d}{d b}
$$

$\therefore$ (1) becomv.

\begin{flalign*}
	 & (D-7)\left(c_{1} e^{s t}+c_{2} e^{s t}\right)+y=0                               \\
	 & \Rightarrow=5 c_{1} e^{s t}+6 c_{2} e^{6 t}-7 c_{1} e^{s t}-7 c_{2} e^{-s t}=-y \\
	 & \Rightarrow y=2 c_{1} e^{s t}+c_{2} e^{6 t}
\end{flalign*}

$$
	\& \quad x=c_{1} e^{5 t}+c_{2} e^{6 t}
$$

$2 \frac{d x}{d t}+2 x-3 y=t \quad, \quad \frac{d y}{d t}-3 x+2 y=e^{2 t}$

A)


\begin{align*}
	 & (D+2) x-3 y=t                                             \\
	 & (D+2) \text{ y }-3 x=e^{2 t}  \tag{2}                     \\
	 & \text{ (1) } \times 3: 8                                  \\
	 & 3 x(D+2)-9 y=3 t  \tag{3}                                 \\
	 & +\left(-3 x(D+2)+(D+2)^{2} y=(D+2) e^{2 t}\right) \tag{9}
\end{align*}


(3) + (4)

\begin{flalign*}
	 & y\left((D+2)^{2}-4\right)=3 t+4 e^{2 t}                   \\
	 & y\left(D^{2}+4 D-5\right)=3 t+4 e^{2 t}                   \\
	 & =y(D+5)(D-1) \cdot                                        \\
	 & \therefore \quad \text{ roots }=-5,+1                     \\
	 & \therefore C F_{\text{an } y} c_{1} e^{-5 t}+C_{2} e^{+t}
\end{flalign*}

\begin{flalign*}
	P I_{y_{1}}=  & \frac{3 t}{\left(D^{2}+4 D-5\right)}                                                  \\
	              & =-\frac{3}{5} \times\left(1+\left(\frac{D^{2}}{-5}-\frac{4}{5} D\right)\right)^{-1} t \\
	              & =-\frac{3}{5} \times\left(1-\frac{D^{2}}{-5}+\frac{4}{5} D x^2 +\cdots\right) t       \\
	              & =-\frac{3}{5}\left(t+0+\frac{4}{5}\right)                                             \\
	P I_{y_{1}}=  & \frac{4 e^{2 t}}{(D+5)(D-1)}                                                          \\
	\Rightarrow   & \frac{4}{7} t-\frac{12}{25}                                                           \\
	\Rightarrow y & =C F_{y}+P I_{y_{1}}+P I_{y_{2}}                                                      \\
	\therefore y  & =C_{1} e^{-5 t}+C_{2} e^{t}-\frac{3}{5} t+\frac{4}{7} e^{2 t}-\frac{12}{25}
\end{flalign*}

Substitute in (2):

\begin{flalign*}
	 & (D+2) y-e^{2 t}=3 x \Rightarrow x=\frac{1}{3}\left[(D+2) y-\frac{t}{2} e^{2 t}\right]                    \\
	 & x=\frac{1}{3}\left(-5 c_{1} e^{-5 t}+c_{2} e^{t}-\frac{3}{5}+\frac{8}{7} e^{2 t}\right.                  \\
	 & \left.+2 c_{1} e^{-5 t}+2 c_{2} e^{t}-\frac{6}{5} t+\frac{8}{7} e^{2 t}-\frac{24}{25}-e^{2 t}\right)     \\
	 & =\frac{1}{3}\left(-3 c_{1} e^{-5 t}+3 c_{2} e^{t}+\frac{9}{7} e^{2 t}-\frac{6}{5} t-\frac{39}{25}\right)
\end{flalign*}

$$
	x=-c_1 e^{-5 t}+c_2 e^t+\frac{3}{7} e^{2 t}-\frac{2}{5} t-\frac{13}{25}
$$
3.
\begin{flalign*}
	 & \frac{d x}{d t}+2 y=-\sin(t), \\
	 & \frac{d y}{d t}=2 x+\cos(t)
\end{flalign*}
A) $\quad \frac{d x}{d t}+2 y=-\sin(t)$-1
\begin{flalign*}
	 & \frac{d x}{d t}+2 y=-\sin(t)-(D)(D-2) x+(D+2) y=\cos(t)-\sin(t) \\
	 & \frac{d y}{d t}-2 x=\cos(t) \quad \text{ (D) }
\end{flalign*}
(1) $\times 2$,
$$
	2 x \cdot 0+4 y=-2 \sin(t)
$$
(2) $\times 0$.
$$
	D^2 \cdot y-2 x \cdot D=D \cdot \cos(t)-(4)
$$
(3) + (4):
\begin{flalign*}
	 & D^2 \cdot y+4 y=-3 \sin(t)                                                                \\
	 & \frac{d^2 y}{d t}+4 y=-3 \sin(t)                                                          \\
	 & \therefore \quad y e^{4 t}=\int e^{4 t} x-3 \sin(t) d t=-3 \int \sin(t) e^{4 t} \cdot d t \\
	 &
\end{flalign*}
\begin{flalign*}
	I          & =-3 \int \sin(t) e^{4 t} d t \quad I_2=\cos(t) 4 e^{44}+\underbrace{4 \int \sin(t) \ldots}        \\
	           & =-3(\sin(t) \times 4 e^{4 t}-4 \underbrace{\cos(t) \cdot e^{4 t}}_I) \quad=40 \cos(t) e^{4 t}+4 I \\
	           & =-8 \sin(t) e^{4 t}+32 \cos(t) e^{4 t}+32 I                                                       \\
	\therefore & =\frac{e^{4 t}}{4^2+1}(4 \sin(t)-\cos(4 t)
\end{flalign*}
$$
	\therefore \quad=\frac{e^{4 t}}{4^2+1}(4 \sin(t)-\cos(\theta t)
$$
or \begin{flalign*}
	\left(p^2+4\right) y=-3 \sin(t) \\
\end{flalign*}
\begin{flalign*}
	 & \therefore y=\left(c_1 \cos(2 t)+c_2 \sin(2 t)\right) \\
	 & P I=\frac{-3 \sin(t)}{D^2+4}, \quad D^2=-1            \\
	 & \Rightarrow-\frac{3}{3} \sin(t)=-\sin(t)              \\
	 & \therefore y=c_1 \cos(2 t)+c_2 \sin(2 t)-\sin(t)
\end{flalign*}

Substitute this in (2):
\begin{flalign*}
	 & \begin{array}{l}
		   \Rightarrow x=-e^{2 t}\left(\cos ^5\left(-c_1+c_2\right)\right. \\
		   \left.\Rightarrow x=-2 e^{2 t}\left(c_1+c_2\right) \cos(2 t)+\left(c_2-c_1\right) \sin(2 E)\right)-\frac{1}{16}-\cos(t)
	   \end{array} \\
	 & 2=-\frac{1}{2}\left(\cos(t)-2 c_1 \sin(2 t)+2 c_2 \cos(2 t)-\sin(t)\right)                                                                               \\
	 &
\end{flalign*}

Hew
1. $\frac{d y}{d t}+2 y+x=\sin(t) \quad \frac{d x}{d t}-4 y-2 x=\cos(t)$
H)
\begin{flalign*}
	 & D y+2 y+x=\sin(t)   \\
	 & D x-4 y-2 x=\cos(t)
\end{flalign*}
$\mathcal{C} \times \bar{\partial} D:$
\begin{flalign*}
	 & -D^2 y+2 D y-D x=-\cos(t)                      \\
	 & \oplus-4 y+D x-42 x=\sin(t)                    \\
	 & -\left(+D^2+2 D+4\right) y-2 x=\sin(t)-\cos(t)
\end{flalign*}
(20) 2
\begin{flalign*}
	 & \therefore+\frac{2 D y+4 y+2 x=2 \sin(t)}{\left.4 D^2+3\right)} \\
	 & -D^2 y=3 \sin(t)-\cos(t)                                        \\
	 & \therefore y=\int(\cos(t)-3 \sin(t)) d t d t                    \\
	 & =\int(\sin(t)+3 \cos(t)) d t                                    \\
	 & y=3 \sin(t) \cos(t) \quad y=2 \sin(t)+c t+2
\end{flalign*}
$\therefore$ from (0:
$8 \sin(t)+B 3 \cos(t)+266 \sin(t)-2 \cos(t)+x=\sin(t)$
$\therefore x=-6 \sin(t)-\cos(t) \quad x=-3 \sin(t)-2 \cos(\theta$
$$
	-2 c t+2 c_2+c
$$
